pulse/lib/steel/pulse/Pulse.Checker.While.fst
@@ -10,7 +10,7 @@ open Pulse.Checker.Common
 
 module P = Pulse.Syntax.Printer
 module FV = Pulse.Typing.FV
-
+module Framing = Pulse.Checker.Framing
 module Metatheory = Pulse.Typing.Metatheory
 
 let while_cond_comp_typing (#g:env) (u:universe) (ty:term) (inv_body:term)
@@ -38,63 +38,68 @@ let check_while
   let g = push_context "while loop" g in
   let Tm_While { invariant=inv; condition=cond; body } = t.term in
   let (| ex_inv, inv_typing |) =
-    check_vprop (push_context "invariant" g) (Tm_ExistsSL u0 tm_bool inv should_elim_true) in
-  match ex_inv with
-  | Tm_ExistsSL u ty inv _ ->
-    if not (eq_tm ty tm_bool) ||
-       not (eq_univ u u0)
-    then T.fail "While loop invariant is exists but its witness type is not bool"
-    else begin
-      let while_cond_comp_typing = while_cond_comp_typing u ty inv inv_typing in
-      let (| res_typing, cond_pre_typing, x, post_typing |) =
-          Metatheory.(st_comp_typing_inversion (comp_typing_inversion while_cond_comp_typing))
-      in
-      let while_cond_hint
-        : post_hint_for_env g
-        = post_hint_from_comp_typing while_cond_comp_typing
-      in
-      let (| cond, cond_comp, cond_typing |) =
-        check' allow_inst
-               (push_context "while condition" g)
-               cond
-               (comp_pre (comp_while_cond inv))
-               cond_pre_typing
-               (Some while_cond_hint)
-      in
-      if eq_comp cond_comp (comp_while_cond inv)
-      then begin
-        let while_body_comp_typing = while_body_comp_typing u ty inv inv_typing in
-        let (| res_typing, body_pre_typing, x, post_typing |) = 
-            Metatheory.(st_comp_typing_inversion (comp_typing_inversion while_body_comp_typing))
+    check_vprop (push_context "invariant" g)
+                (Tm_ExistsSL u0 tm_bool inv should_elim_true)
+  in
+  match Framing.check_frameable pre_typing ex_inv with
+  | Inr f -> T.raise (Framing_failure f)
+  | Inl framing_token ->
+    match ex_inv with
+    | Tm_ExistsSL u ty inv _ ->
+      if not (eq_tm ty tm_bool) ||
+        not (eq_univ u u0)
+      then T.fail "While loop invariant is exists but its witness type is not bool"
+      else begin
+        let while_cond_comp_typing = while_cond_comp_typing u ty inv inv_typing in
+        let (| res_typing, cond_pre_typing, x, post_typing |) =
+            Metatheory.(st_comp_typing_inversion (comp_typing_inversion while_cond_comp_typing))
         in
-        let while_post_hint
+        let while_cond_hint
           : post_hint_for_env g
-          = post_hint_from_comp_typing while_body_comp_typing
+          = post_hint_from_comp_typing while_cond_comp_typing
         in
-        let (| body, body_comp, body_typing |) =
-            check' allow_inst
-                   (push_context "while body" g)
-                   body
-                   (comp_pre (comp_while_body inv))
-                   body_pre_typing
-                   (Some while_post_hint)
+        let (| cond, cond_comp, cond_typing |) =
+          check' allow_inst
+                 (push_context "while condition" g)
+                 cond
+                 (comp_pre (comp_while_cond inv))
+                 cond_pre_typing
+                 (Some while_cond_hint)
         in
-        if eq_comp body_comp (comp_while_body inv)
-        then let d = T_While g inv cond body inv_typing cond_typing body_typing in
-             repack (try_frame_pre pre_typing d) post_hint true
-        else 
-          T.fail
-            (Printf.sprintf "Could not prove the inferred type of the while body matches the annotation\n\
-                                   Inferred type = %s\n\
-                                   Annotated type = %s\n"
-                                   (P.comp_to_string body_comp)
-                                   (P.comp_to_string (comp_while_body inv)))
-    end
-    else T.fail 
-           (Printf.sprintf "Could not prove that the inferred type of the while condition matches the annotation\n\
-                            Inferred type = %s\n\
-                            Annotated type = %s\n"
-                            (P.comp_to_string cond_comp)
-                            (P.comp_to_string (comp_while_cond inv)))
-    end
-  | _ -> T.fail "Typechecked invariant is not an exists"
+        if eq_comp cond_comp (comp_while_cond inv)
+        then begin
+          let while_body_comp_typing = while_body_comp_typing u ty inv inv_typing in
+          let (| res_typing, body_pre_typing, x, post_typing |) = 
+              Metatheory.(st_comp_typing_inversion (comp_typing_inversion while_body_comp_typing))
+          in
+          let while_post_hint
+            : post_hint_for_env g
+            = post_hint_from_comp_typing while_body_comp_typing
+          in
+          let (| body, body_comp, body_typing |) =
+              check' allow_inst
+                     (push_context "while body" g)
+                     body
+                     (comp_pre (comp_while_body inv))
+                     body_pre_typing
+                     (Some while_post_hint)
+          in
+          if eq_comp body_comp (comp_while_body inv)
+          then let d = T_While g inv cond body inv_typing cond_typing body_typing in
+               repack (Framing.apply_frame pre_typing d framing_token) post_hint true
+          else 
+            T.fail
+              (Printf.sprintf "Could not prove the inferred type of the while body matches the annotation\n\
+                                     Inferred type = %s\n\
+                                     Annotated type = %s\n"
+                                     (P.comp_to_string body_comp)
+                                     (P.comp_to_string (comp_while_body inv)))
+      end
+      else T.fail 
+(Printf.sprintf "Could not prove that the inferred type of the while condition matches the annotation\n\
+                                 Inferred type = %s\n\
+                                 Annotated type = %s\n"
+                                 (P.comp_to_string cond_comp)
+                                 (P.comp_to_string (comp_while_cond inv)))
+                end
+     | _ -> T.fail "Typechecked invariant is not an exists"
